aesop navigation

Examples2.lean
@@ -1,4 +1,107 @@
 import PBN
+import Aesop
+
+--set_option trace.aesop.tree true
+--set_option trace.Elab.definition true
+set_option pp.all true
+
+
+
+set_option aesop.check.all true
+
+/-abbrev Variable := String
+
+def State := Variable → Nat
+
+inductive Stmt : Type where
+  | skip : Stmt
+  | assign : Variable → (State → Nat) → Stmt
+  | seq : Stmt → Stmt → Stmt
+  | ifThenElse : (State → Prop) → Stmt → Stmt → Stmt
+  | whileDo : (State → Prop) → Stmt → Stmt
+
+infix:60 ";; " => Stmt.seq
+
+export Stmt (skip assign seq ifThenElse whileDo)
+
+set_option quotPrecheck false in
+notation s:70 "[" x:70 "↦" n:70 "]" => (fun v ↦ if v = x then n else s v)
+
+inductive BigStep : Stmt → State → State → Prop where
+  | protected skip (s : State) :
+    BigStep skip s s
+  | protected assign (x : Variable) (a : State → Nat) (s : State) :
+    BigStep (assign x a) s (s[x ↦ a s])
+  | protected seq {S T : Stmt} {s t u : State} (hS : BigStep S s t) (hT : BigStep T t u) :
+    BigStep (S;; T) s u
+  | protected if_true {B : State → Prop} {s t : State} (hcond : B s) (S T : Stmt) (hbody : BigStep S s t) :
+    BigStep (ifThenElse B S T) s t
+  | protected if_false {B : State → Prop} {s t : State} (hcond : ¬ B s) (S T : Stmt) (hbody : BigStep T s t) :
+    BigStep (ifThenElse B S T) s t
+  | while_true {B S s t u} (hcond : B s) (hbody : BigStep S s t) (hrest : BigStep (whileDo B S) t u) :
+    BigStep (whileDo B S) s u
+  | while_false {B S s} (hcond : ¬ B s) :
+    BigStep (whileDo B S) s s
+
+notation:55 "(" S:55 "," s:55 ")" " ⇓ " t:55 => BigStep S s t
+
+add_aesop_rules safe [BigStep.skip, BigStep.assign, BigStep.seq, BigStep.while_false]
+add_aesop_rules 50% [apply BigStep.while_true]
+add_aesop_rules safe [
+  (by apply BigStep.if_true (hcond := by assumption) (hbody := by assumption)),
+  (by apply BigStep.if_false (hcond := by assumption) (hbody := by assumption))
+]
+
+@[aesop unsafe]
+theorem state_extensionality {S : Stmt} {s1 s2 t : State}
+  (eq: ∀ v, s1 v = s2 v) (h : (S, s1) ⇓ t) : (S, s2) ⇓ t :=
+  by
+    have h : s1 = s2 := by funext; aesop
+    aesop
+
+namespace BigStep
+
+--@[aesop safe destruct]
+--theorem cases_if_of_true {B S T s t} (hcond : B s) : (ifThenElse B S T, s) ⇓ t → (S, s) ⇓ t := by
+  --intro h; cases h <;> aesop
+
+@[aesop safe destruct]
+theorem cases_if_of_false {B S T s t} (hcond : ¬ B s) : (ifThenElse B S T, s) ⇓ t → (T, s) ⇓ t := by
+  intro h; cases h <;> aesop
+
+@[aesop 30%]
+theorem and_excluded {P Q R : Prop} (hQ : P → Q) (hR : ¬ P → R) : (P ∧ Q ∨ ¬ P ∧ R) := by
+  by_cases h : P <;> aesop
+
+theorem if_iff {B S T s t} : (ifThenElse B S T, s) ⇓ t ↔
+    (B s ∧ (S, s) ⇓ t) ∨ (¬ B s ∧ (T, s) ⇓ t) := by
+    navaesop "A!" (BigStep S s t)
+
+  --aesop
+  --navaesop
+
+
+end BigStep-/
+
+
+
+
+
+
+
+
+
+
+
+
+
+
+
+
+
+
+
+
 
 theorem testinggg (a b c d u w y z : Prop) (f : b → c → a) (g : c → d → a) (x : w → d) (j : a → u → y):
     y :=
@@ -8,11 +111,39 @@ theorem testinggg (a b c d u w y z : Prop) (f : b → c → a) (g : c → d → 
 
   navhavent c
 
-theorem ao_example2 (A B C D M E X Z Y P : Prop) (f : B → C → A) (g : C → D → M → A) (h : E → X → Z → B) (i : Z → Y → P → B) :
+theorem exists_five : ∃ n : Nat, n = 5 := by
+  apply Exists.intro
+
+
+theorem ao_exampleee (A B C D M E X Z Y P Q L : Prop) (f : B → C → Q → L → A) (g : C → B → A) (h : E → X → Z → B) (i : Z → Y → P → B) (j : M → D) (hX : X) (hZ : Z) :
     A :=
   by
+
+
+theorem ao_example2 (A B C D M E X Z Y P Q L : Prop) (g : C → B → A) (h : X → Z → B) (i : Z → Y → P → B) (j : M → D) (hX : X) (hZ : Z) :
+    A :=
+  by
+  --have hC : C := ?_
+  --aesop
+  navaesop "C" C
+  --have hM : M := ?_
+
+
+
+  --navaesop
+  --navaesop
+  --aesop
+  /-navhave hM : M end
+  navhave hQ : Q end
+  navaesop
+  aesop
+
+
+
   navhave hC : C end
   navhave! hB : B end
+
+
   . sorry
   . navhave! hZ : Z end
     navhave hY : Y end
@@ -21,7 +152,7 @@ theorem ao_example2 (A B C D M E X Z Y P : Prop) (f : B → C → A) (g : C → 
     navhave hE : E end
     . sorry
     . sorry
-    . sorry
+    . sorry-/
 
   /-
     navhave hC : C end
@@ -43,6 +174,39 @@ theorem more_nonsense (a b c : Prop) :
   navhave hab : a → b end
   . intro ha
     exact hb
+
+
+
+theorem weak_peirce (a b : Prop) :
+    ((((a → b) → a) → a) → b) → b := by
+  sorry
+
+theorem about_Impl (a b : Prop) :
+  ¬ a ∨ b → a → b := by
+  intro f ha
+  navhave na : ¬a end
+
+
+def ExcludedMiddle : Prop :=
+  ∀a : Prop, a ∨ ¬ a
+
+def Peirce : Prop :=
+  ∀a b : Prop, ((a → b) → a) → a
+
+def DoubleNegation : Prop :=
+  ∀a : Prop, (¬¬ a) → a
+
+theorem EM_of_DN : DoubleNegation → ExcludedMiddle := by
+  --printAndOrGraph
+  unfold DoubleNegation
+  unfold ExcludedMiddle
+  intro dn a
+
+  --apply dn
+  --intro n
+
+
+
 
 
 
@@ -69,3 +233,4 @@ theorem more_nonsense (a b c : Prop) :
 -- how much to take into account that the lean context can have new rules added in the middle of a proof?
 
 -- how much does it matter what is displayed in the context vs the state of the and/or graph? Like when y is leftover from a navhavnet y because it wasn't in the and/or graph?
+-- what if context needs to be massaged through intros and such?
