PBN/SimpleAndOrGraphs.lean
@@ -1,0 +1,75 @@
+-- Build and traverse AND-OR graphs
+import Lean
+import Std.Data.HashMap
+import Std.Data.HashSet
+
+open Std
+open Lean Lean.Elab.Tactic
+open Lean Elab Tactic Meta
+
+-- T
+-- T! : prune
+-- A! : prune and axiomotize
+-- A : axiomotize
+-- F : prune
+
+structure SimpleANDORGraph where
+  or_nodes : List (String × String)
+  edges : List (String × String)
+
+-- return the conclusion of an AND-node (its parent)
+def conclusion (graph : SimpleANDORGraph) (and_node : String) : MetaM String := do
+  for edge in graph.edges do
+    if edge.2 == and_node then
+      return edge.1
+  throwError "no parent"
+
+-- return consumers of an OR-node (all of its parents)
+def consumers (graph : SimpleANDORGraph) (or_node : String) : MetaM (List String) := do
+  let mut consumers : List String := []
+  for edge in graph.edges do
+    if edge.2 == or_node then
+      consumers := edge.1 :: consumers
+  return consumers
+
+-- return premises of an AND-node
+def premises (graph : SimpleANDORGraph) (and_node : String) : MetaM (List String) := do
+  let mut ps := []
+  for edge in graph.edges do
+    if edge.1 == and_node then
+      ps := edge.2 :: ps
+  return ps
+
+def provableORNodes (graph : SimpleANDORGraph) (and_leaves : List String) : MetaM (List String) := do
+  let mut inferred : HashSet String := {}
+  let mut agenda : List (MetaM String) :=  and_leaves.map (conclusion graph)
+  let mut count : HashMap String Nat := {}
+
+  while agenda.length > 0 do
+    let p ← agenda.head!
+    agenda := agenda.tail
+    if inferred.contains p then
+      continue
+
+    inferred := inferred.insert p
+
+    for consumer in (← consumers graph p) do
+      -- if consumer is not in count, add to count and initialize value to # args it consumes
+      if !count.contains consumer then
+        count := count.insert consumer (← premises graph consumer).length
+
+      let c : Nat := count.get! consumer
+      count := count.insert consumer (c - 1)
+
+      -- if value is 0, all args have been proven
+      if c - 1 == 0 then
+        agenda := conclusion graph consumer :: agenda
+
+  return inferred.toList
+
+-- is an OR-node provable?
+def provable (graph : SimpleANDORGraph) (and_leaves : List String) (or_node : String) : MetaM Bool := do
+  let provable_or_nodes ← provableORNodes graph and_leaves
+  logInfo m!"and_leaves : {and_leaves}"
+  logInfo m!"provable or nodes : {provable_or_nodes}"
+  return provable_or_nodes.contains or_node
